wip: exp_fw

code/bignum/Hacl.Spec.Bignum.ExponentiationPrecomp.fst
@@ -200,16 +200,41 @@ val bn_mod_precomp_table_mont_loop_lemma:
     index t02 0 == bn_v (sub t01 0 nLen) /\
     index t02 1 == bn_v (sub t01 nLen nLen))
   (ensures
-   (let t3 : lbignum t (table_len * nLen) = Loops.repeati j (bn_mod_precomp_table_mont_f n mu aM table_len) t01 in
-    let t4 : lseq nat table_len = Loops.repeati j
-      (E.mod_precomp_table_mont_f (bits t) nLen (bn_v n) (v mu) (bn_v aM) table_len) t02 in
+   (let t1: lbignum t (table_len * nLen) = Loops.repeati j (bn_mod_precomp_table_mont_f n mu aM table_len) t01 in
+    let t2: lseq nat table_len = Loops.repeati j (E.mod_precomp_table_mont_f (bits t) nLen (bn_v n) (v mu) (bn_v aM) table_len) t02 in
     (forall (i:nat{i < j + 2}).
-     (Math.Lemmas.lemma_mult_le_right nLen (i + 1) (table_len);
+     (Math.Lemmas.lemma_mult_le_right nLen (i + 1) table_len;
       assert (i * nLen + nLen <= table_len * nLen);
-      let bi = sub t3 (i * nLen) nLen in bn_v bi == index t4 i /\ bn_v bi < bn_v n))))
+      let bi = sub t1 (i * nLen) nLen in bn_v bi == index t2 i))))
 
-let bn_mod_precomp_table_mont_loop_lemma #t #nLen n mu table_len aM t01 t02 j =
-  admit()
+let rec bn_mod_precomp_table_mont_loop_lemma #t #nLen n mu table_len aM t01 t02 j = admit()
+  // let t1: lbignum t (table_len * nLen) = Loops.repeati j (bn_mod_precomp_table_mont_f n mu aM table_len) t01 in
+  // let t2: lseq nat table_len = Loops.repeati j (E.mod_precomp_table_mont_f (bits t) nLen (bn_v n) (v mu) (bn_v aM) table_len) t02 in
+
+  // if j = 0 then begin
+  //   Loops.eq_repeati0 j (bn_mod_precomp_table_mont_f n mu aM table_len) t01;
+  //   Loops.eq_repeati0 j (E.mod_precomp_table_mont_f (bits t) nLen (bn_v n) (v mu) (bn_v aM) table_len) t02;
+  //   () end
+  // else begin
+  //   let t3: lbignum t (table_len * nLen) = Loops.repeati (j - 1) (bn_mod_precomp_table_mont_f n mu aM table_len) t01 in
+  //   let t4: lseq nat table_len = Loops.repeati (j - 1) (E.mod_precomp_table_mont_f (bits t) nLen (bn_v n) (v mu) (bn_v aM) table_len) t02 in
+
+  //   Loops.unfold_repeati j (bn_mod_precomp_table_mont_f n mu aM table_len) t01 (j - 1);
+  //   Loops.unfold_repeati j (E.mod_precomp_table_mont_f (bits t) nLen (bn_v n) (v mu) (bn_v aM) table_len) t02 (j - 1);
+  //   bn_mod_precomp_table_mont_loop_lemma n mu table_len aM t01 t02 (j - 1);
+
+  //   // assert (forall (i:nat{i < j + 1}).
+  //   //  (Math.Lemmas.lemma_mult_le_right nLen (i + 1) (table_len);
+  //   //   assert (i * nLen + nLen <= table_len * nLen);
+  //   //   let bi = sub t3 (i * nLen) nLen in bn_v bi == index t4 i));
+
+  //   // assert (index t2 (j + 1) == M.mont_mul (bits t) nLen (bn_v n) (v mu) t4.[j] (bn_v aM));
+
+  //   assume (forall (i:nat{i < j + 2}).
+  //    (Math.Lemmas.lemma_mult_le_right nLen (i + 1) (table_len);
+  //     assert (i * nLen + nLen <= table_len * nLen);
+  //     let bi = sub t1 (i * nLen) nLen in bn_v bi == index t2 i));
+  //   () end
 
 
 val bn_mod_precomp_table_mont_lemma:
@@ -243,7 +268,21 @@ let bn_mod_precomp_table_mont_lemma #t #nLen n mu table_len aM oneM i =
   LSeq.eq_intro (sub t01 0 nLen) (sub t01' 0 nLen);
   assert (index t02 0 == bn_v (sub t01 0 nLen));
   assert (index t02 1 == bn_v (sub t01 nLen nLen));
-  bn_mod_precomp_table_mont_loop_lemma #t #nLen n mu table_len aM t01 t02 (table_len - 2)
+  bn_mod_precomp_table_mont_loop_lemma n mu table_len aM t01 t02 (table_len - 2);
+
+  let t1 : lbignum t (table_len * nLen) = bn_mod_precomp_table_mont n mu table_len aM oneM in
+  let t2 : lseq nat table_len = E.mod_precomp_table_mont (bits t) nLen (bn_v n) (v mu) table_len (bn_v aM) in
+
+  Math.Lemmas.lemma_mult_le_right nLen (i + 1) (table_len);
+  assert (i * nLen + nLen <= table_len * nLen);
+  let bi = sub t1 (i * nLen) nLen in
+  assert (bn_v bi == index t2 i);
+
+  bn_eval_bound n nLen;
+  M.mont_preconditions (bits t) nLen (bn_v n) (v mu);
+  assert (E.mont_pre (bits t) nLen (bn_v n) (v mu));
+  E.mod_precomp_table_mont_lemma (bits t) nLen (bn_v n) (v mu) table_len (bn_v aM) i;
+  assert (bn_v bi < bn_v n)
 
 
 val bn_mod_exp_fw_mont_f_lemma:
@@ -258,8 +297,8 @@ val bn_mod_exp_fw_mont_f_lemma:
   -> table_len:size_nat{1 < table_len /\ table_len * nLen <= max_size_t /\ table_len == pow2 l}
   -> oneM:lbignum t nLen
   -> aM:lbignum t nLen
-  -> i:nat{l * (i + 1) <= bBits}
-  -> accM:lbignum t nLen -> Lemma
+  -> accM:lbignum t nLen
+  -> i:nat{l * (i + 1) <= bBits} -> Lemma
   (requires
     BM.bn_mont_pre n mu /\ bn_v aM < bn_v n /\
     bn_v accM < bn_v n /\ bn_v b < pow2 bBits /\
@@ -272,13 +311,9 @@ val bn_mod_exp_fw_mont_f_lemma:
     let r2 = E.mod_exp_fw_mont_f (bits t) nLen (bn_v n) (v mu) bBits (bn_v b) l table_len t2 i (bn_v accM) in
     bn_v r1 == r2 /\ bn_v r1 < bn_v n))
 
-let bn_mod_exp_fw_mont_f_lemma #t #nLen n mu bBits bLen b l table_len oneM aM i accM =
+let bn_mod_exp_fw_mont_f_lemma #t #nLen n mu bBits bLen b l table_len oneM aM accM i =
   let t1 = bn_mod_precomp_table_mont n mu table_len aM oneM in
   let t2 = E.mod_precomp_table_mont (bits t) nLen (bn_v n) (v mu) table_len (bn_v aM) in
-
-  let acc_pow2l = bn_mod_exp_pow2_mont n mu accM l in
-  bn_mod_exp_pow2_mont_lemma n mu accM l;
-  assert (bn_v acc_pow2l < bn_v n);
 
   let bits_l = BN.bn_get_bits b (bBits - l * i - l) l in
   BN.bn_get_bits_lemma b (bBits - l * i - l) l;
@@ -290,6 +325,10 @@ let bn_mod_exp_fw_mont_f_lemma #t #nLen n mu bBits bLen b l table_len oneM aM i 
   let a_powbits_l = sub t1 (v bits_l * nLen) nLen in
   bn_mod_precomp_table_mont_lemma n mu table_len aM oneM (v bits_l);
   assert (bn_v a_powbits_l < bn_v n);
+
+  let acc_pow2l = bn_mod_exp_pow2_mont n mu accM l in
+  bn_mod_exp_pow2_mont_lemma n mu accM l;
+  assert (bn_v acc_pow2l < bn_v n);
 
   let res = BM.bn_mont_mul n mu acc_pow2l a_powbits_l in
   BM.bn_mont_mul_lemma n mu acc_pow2l a_powbits_l
@@ -347,7 +386,117 @@ let bn_mod_exp_fw_mont_rem_lemma #t #nLen n mu bBits bLen b l table_len oneM aM 
   BM.bn_mont_mul_lemma n mu acc_pow2c a_powbits_c
 
 
-let bn_mod_exp_fw_precompr2_lemma #t nLen n a bBits b l r2 = admit()
+// val bn_mod_exp_fw_mont_loop_lemma:
+//     #t:limb_t
+//   -> #nLen:size_pos{nLen + nLen <= max_size_t}
+//   -> n:lbignum t nLen
+//   -> mu:limb t
+//   -> aM:lbignum t nLen
+//   -> bBits:size_pos
+//   -> b:lbignum t (blocks bBits (bits t))
+//   -> l:size_pos{l <= bits t}
+//   -> table_len:size_nat{1 < table_len /\ table_len * nLen <= max_size_t /\ table_len == pow2 l}
+//   -> oneM:lbignum t nLen
+//   -> accM0:lbignum t nLen
+//   -> j:nat{l * j <= bBits} -> Lemma
+//   (requires
+//     BM.bn_mont_pre n mu /\ bn_v aM < bn_v n /\
+//     bn_v accM0 < bn_v n /\ bn_v b < pow2 bBits /\
+//     bn_v oneM == M.to_mont (bits t) nLen (bn_v n) (v mu) 1)
+//   (ensures
+//    (let t1 = bn_mod_precomp_table_mont n mu table_len aM oneM in
+//     let t2 = E.mod_precomp_table_mont (bits t) nLen (bn_v n) (v mu) table_len (bn_v aM) in
+//     let bLen = blocks bBits (bits t) in
+
+//     let accM1: lbignum t nLen = Loops.repeati j (bn_mod_exp_fw_mont_f n mu bBits bLen b l table_len t1) accM0 in
+//     let accM2 = Loops.repeati j (E.mod_exp_fw_mont_f (bits t) nLen (bn_v n) (v mu) bBits (bn_v b) l table_len t2) (bn_v accM0) in
+//     bn_v accM1 == accM2 /\ bn_v accM1 < bn_v n))
+
+// let bn_mod_exp_fw_mont_loop_lemma #t #nLen n mu aM bBits b l table_len oneM accM0 j =
+  // let t1 = bn_mod_precomp_table_mont n mu table_len aM oneM in
+  // let t2 = E.mod_precomp_table_mont (bits t) nLen (bn_v n) (v mu) table_len (bn_v aM) in
+  // let bLen = blocks bBits (bits t) in
+
+  // if j = 0 then begin
+  //   Loops.eq_repeati0 j (bn_mod_exp_fw_mont_f n mu bBits bLen b l table_len t1) accM0;
+  //   Loops.eq_repeati0 j (E.mod_exp_fw_mont_f (bits t) nLen (bn_v n) (v mu) bBits (bn_v b) l table_len t2) (bn_v accM0) end
+  // else begin
+  //   Math.Lemmas.lemma_mult_lt_left l (j - 1) j;
+  //   let accM4 = Loops.repeati (j - 1) (bn_mod_exp_fw_mont_f n mu bBits bLen b l table_len t1) accM0 in
+  //   Loops.unfold_repeati j (E.mod_exp_fw_mont_f (bits t) nLen (bn_v n) (v mu) bBits (bn_v b) l table_len t2) (bn_v accM0) (j - 1);
+  //   Loops.unfold_repeati j (bn_mod_exp_fw_mont_f n mu bBits bLen b l table_len t1) accM0 (j - 1);
+  //   bn_mod_exp_fw_mont_loop_lemma n mu aM bBits b l table_len oneM accM0 (j - 1);
+  //   bn_mod_exp_fw_mont_f_lemma n mu bBits bLen b l table_len oneM aM accM4 (j - 1);
+  //   () end
+
+
+val bn_mod_exp_fw_mont_aux_lemma:
+    #t:limb_t
+  -> #nLen:size_pos{nLen + nLen <= max_size_t}
+  -> n:lbignum t nLen
+  -> mu:limb t
+  -> aM:lbignum t nLen
+  -> bBits:size_pos
+  -> b:lbignum t (blocks bBits (bits t))
+  -> l:size_pos{l <= bits t /\ pow2 l * nLen <= max_size_t}
+  -> r2:lbignum t nLen -> Lemma
+  (requires
+    BM.bn_mont_pre n mu /\ bn_v aM < bn_v n /\ bn_v b < pow2 bBits /\
+    bn_v r2 == pow2 (2 * bits t * nLen) % bn_v n)
+  (ensures
+   (let r1 = bn_mod_exp_fw_mont_ n mu aM bBits b l r2 in
+    let r2 = E.mod_exp_fw_mont_ (bits t) nLen (bn_v n) (v mu) (bn_v aM) bBits (bn_v b) l in
+    bn_v r1 == r2 /\ bn_v r1 < bn_v n))
+
+let bn_mod_exp_fw_mont_aux_lemma #t #nLen n mu aM bBits b l r2 =
+  let bLen = blocks bBits (bits t) in
+  let one = BN.bn_from_uint nLen (uint #t 1) in
+  BN.bn_from_uint_lemma nLen (uint #t 1);
+  assert (bn_v one = 1);
+
+  let oneM = BM.bn_to_mont n mu r2 one in
+  BM.bn_to_mont_lemma n mu r2 one;
+  assert (bn_v oneM == M.to_mont (bits t) nLen (bn_v n) (v mu) (bn_v one) /\ bn_v oneM < bn_v n);
+
+  let table_len = pow2 l in
+  Math.Lemmas.pow2_le_compat l 1;
+  assert (1 < table_len /\ table_len * nLen <= max_size_t);
+
+  let table = bn_mod_precomp_table_mont n mu table_len aM oneM in
+  Math.Lemmas.multiply_fractions bBits l;
+  let accM: lbignum t nLen = Loops.repeati (bBits / l) (bn_mod_exp_fw_mont_f n mu bBits bLen b l table_len table) oneM in
+  admit();
+  //bn_mod_exp_fw_mont_loop_lemma n mu aM bBits b l table_len oneM oneM (bBits / l);
+  //let res = if bBits % l = 0 then accM else bn_mod_exp_fw_mont_rem n mu bBits bLen b l table_len table accM in
+  if bBits % l = 0 then ()
+  else bn_mod_exp_fw_mont_rem_lemma n mu bBits bLen b l table_len oneM aM accM
+
+
+let bn_mod_exp_fw_precompr2_lemma #t nLen n a bBits b l r2 =
+  let mu = BI.mod_inv_limb n.[0] in
+  bn_eval_index n 0;
+  assert (bn_v n % pow2 (bits t) == v n.[0]);
+  Math.Lemmas.pow2_modulo_modulo_lemma_1 (bn_v n) 2 (bits t);
+  assert (v n.[0] % 2 = 1); // since bn_v n % 2 = 1
+  BI.mod_inv_limb_lemma n.[0];
+  assert (BM.bn_mont_pre n mu);
+
+  let aM = BM.bn_to_mont n mu r2 a in
+  BM.bn_to_mont_lemma n mu r2 a;
+  assert (bn_v aM == M.to_mont (bits t) nLen (bn_v n) (v mu) (bn_v a) /\ bn_v aM < bn_v n);
+
+  let resM = bn_mod_exp_fw_mont_ n mu aM bBits b l r2 in
+  bn_mod_exp_fw_mont_aux_lemma n mu aM bBits b l r2;
+  assert (bn_v resM == E.mod_exp_fw_mont_ (bits t) nLen (bn_v n) (v mu) (bn_v aM) bBits (bn_v b) l);
+
+  let res = BM.bn_from_mont n mu resM in
+  BM.bn_from_mont_lemma n mu resM;
+  assert (bn_v res == M.from_mont (bits t) nLen (bn_v n) (v mu) (bn_v resM) /\ bn_v res < bn_v n);
+
+  bn_eval_bound n nLen;
+  M.mont_preconditions (bits t) nLen (bn_v n) (v mu);
+  assert (E.mont_pre (bits t) nLen (bn_v n) (v mu));
+  E.mod_exp_fw_mont_lemma (bits t) nLen (bn_v n) (v mu) (bn_v a) bBits (bn_v b) l
 
 
 let bn_mod_exp_fw #t nLen nBits n a bBits b l =
