code/bignum/Hacl.Bignum.ExponentiationPrecomp.fst
@@ -1,0 +1,316 @@
+module Hacl.Bignum.ExponentiationPrecomp
+
+open FStar.HyperStack
+open FStar.HyperStack.ST
+open FStar.Mul
+
+open Lib.IntTypes
+open Lib.Buffer
+
+open Hacl.Bignum.Definitions
+
+module ST = FStar.HyperStack.ST
+module LSeq = Lib.Sequence
+module Loops = Lib.LoopCombinators
+
+module S = Hacl.Spec.Bignum.ExponentiationPrecomp
+module SN = Hacl.Spec.Bignum
+module SM = Hacl.Spec.Bignum.Montgomery
+
+module BN = Hacl.Bignum
+module BM = Hacl.Bignum.Montgomery
+
+friend Hacl.Spec.Bignum.ExponentiationPrecomp
+
+
+#reset-options "--z3rlimit 150 --fuel 0 --ifuel 0"
+
+inline_for_extraction noextract
+let bn_mod_exp_pow2_mont_in_place_st (t:limb_t) (len:BN.meta_len t) =
+    n:lbignum t len
+  -> mu:limb t
+  -> b:size_t
+  -> res:lbignum t len ->
+  Stack unit
+  (requires fun h ->
+    live h n /\ live h res /\ disjoint n res)
+  (ensures  fun h0 _ h1 -> modifies (loc res) h0 h1 /\
+    as_seq h1 res == S.bn_mod_exp_pow2_mont (as_seq h0 n) mu (as_seq h0 res) (v b))
+
+
+inline_for_extraction noextract
+val bn_mod_exp_pow2_mont_in_place: #t:limb_t -> k:BM.mont t -> bn_mod_exp_pow2_mont_in_place_st t k.BM.bn.BN.len
+let bn_mod_exp_pow2_mont_in_place #t k n mu b res =
+  let h0 = ST.get () in
+  [@ inline_let]
+  let refl h i = as_seq h res in
+  [@ inline_let]
+  let spec h0 = SM.bn_mont_sqr (as_seq h0 n) mu in
+
+  [@ inline_let]
+  let inv h (i:nat{i <= v b}) =
+    modifies1 res h0 h /\
+    live h res /\ live h n /\ disjoint n res /\
+    refl h i == Loops.repeat i (spec h0) (refl h0 0) in
+
+  Loops.eq_repeat0 (spec h0) (refl h0 0);
+  Lib.Loops.for 0ul b inv
+  (fun j ->
+    Loops.unfold_repeat (v b) (spec h0) (refl h0 0) (v j);
+    k.BM.sqr n mu res res)
+
+
+inline_for_extraction noextract
+let bn_mod_precomp_table_mont_f_st (t:limb_t) (len:BN.meta_len t) =
+    n:lbignum t len
+  -> mu:limb t
+  -> aM:lbignum t len
+  -> table_len:size_t{1 < v table_len /\ v table_len * v len <= max_size_t}
+  -> i:size_t{v i < v table_len - 2}
+  -> table:lbignum t (table_len *! len) ->
+  Stack unit
+  (requires fun h ->
+    live h n /\ live h aM /\ live h table /\
+    disjoint table aM /\ disjoint table n /\ disjoint n aM)
+  (ensures  fun h0 _ h1 -> modifies (loc table) h0 h1 /\
+    as_seq h1 table == S.bn_mod_precomp_table_mont_f (as_seq h0 n) mu
+      (as_seq h0 aM) (v table_len) (v i) (as_seq h0 table))
+
+
+inline_for_extraction noextract
+val bn_mod_precomp_table_mont_f: #t:limb_t -> k:BM.mont t -> bn_mod_precomp_table_mont_f_st t k.BM.bn.BN.len
+let bn_mod_precomp_table_mont_f #t k n mu aM table_len i table =
+  [@inline_let] let len : BN.meta_len t = k.BM.bn.BN.len in
+  Math.Lemmas.lemma_mult_lt_right (v len) (v i + 1) (v table_len);
+  Math.Lemmas.lemma_mult_lt_right (v len) (v i + 2) (v table_len);
+  let t1 = sub table ((i +! 1ul) *! len) len in
+  let t2 = sub table ((i +! 2ul) *! len) len in
+  let h0 = ST.get () in
+  [@ inline_let]
+  let spec h0 = SM.bn_mont_mul (as_seq h0 n) mu (as_seq h0 t1) (as_seq h0 aM) in
+
+  update_sub_f h0 table ((i +! 2ul) *! len) len spec
+    (fun _ -> k.BM.mul n mu t1 aM t2);
+  let h1 = ST.get () in
+  assert (as_seq h1 table == LSeq.update_sub (as_seq h0 table) ((v i + 2) * v len) (v len) (spec h0))
+
+
+
+inline_for_extraction noextract
+let bn_mod_precomp_table_mont_st (t:limb_t) (len:BN.meta_len t) =
+    n:lbignum t len
+  -> mu:limb t
+  -> table_len:size_t{1 < v table_len /\ v table_len * v len <= max_size_t}
+  -> aM:lbignum t len
+  -> oneM:lbignum t len
+  -> table:lbignum t (table_len *! len) ->
+  Stack unit
+  (requires fun h ->
+    live h n /\ live h aM /\ live h oneM /\ live h table /\
+    disjoint table oneM /\ disjoint table aM /\ disjoint table n /\
+    disjoint n aM /\ disjoint n oneM /\
+    as_seq h table == LSeq.create (v table_len * v len) (uint #t 0))
+  (ensures  fun h0 _ h1 -> modifies (loc table) h0 h1 /\
+    as_seq h1 table == S.bn_mod_precomp_table_mont (as_seq h0 n) mu (v table_len) (as_seq h0 aM) (as_seq h0 oneM))
+
+
+inline_for_extraction noextract
+val bn_mod_precomp_table_mont: #t:limb_t -> k:BM.mont t -> bn_mod_precomp_table_mont_st t k.BM.bn.BN.len
+let bn_mod_precomp_table_mont #t k n mu table_len aM oneM table =
+  [@inline_let] let len : BN.meta_len t = k.BM.bn.BN.len in
+  update_sub table 0ul len oneM;
+  update_sub table len len aM;
+
+  let h0 = ST.get () in
+  [@ inline_let]
+  let spec h = S.bn_mod_precomp_table_mont_f (as_seq h0 n) mu (as_seq h0 aM) (v table_len) in
+  loop1 h0 (table_len -! 2ul) table spec
+  (fun j ->
+    Loops.unfold_repeati (v table_len - 2) (spec h0) (as_seq h0 table) (v j);
+    bn_mod_precomp_table_mont_f #t k n mu aM table_len j table
+  )
+
+
+inline_for_extraction noextract
+let bn_mod_exp_fw_mont_f_st (t:limb_t) (len:BN.meta_len t) =
+    n:lbignum t len
+  -> mu:limb t
+  -> bBits:size_t{0 < v bBits}
+  -> bLen:size_t{bLen == blocks bBits (size (bits t))}
+  -> b:lbignum t bLen
+  -> l:size_t{v l <= bits t}
+  -> table_len:size_t{1 < v table_len /\ v table_len * v len <= max_size_t /\ v table_len == pow2 (v l)}
+  -> table:lbignum t (table_len *! len)
+  -> i:size_t{v l * (v i + 1) <= v bBits}
+  -> accM:lbignum t len ->
+  Stack unit
+  (requires fun h ->
+    live h n /\ live h b /\ live h table /\ live h accM /\
+    disjoint accM table /\ disjoint accM b /\ disjoint accM n /\
+    disjoint accM n /\ disjoint accM b)
+  (ensures  fun h0 _ h1 -> modifies (loc accM) h0 h1 /\
+    as_seq h1 accM == S.bn_mod_exp_fw_mont_f (as_seq h0 n) mu (v bBits) (v bLen) (as_seq h0 b)
+      (v l) (v table_len) (as_seq h0 table) (v i) (as_seq h0 accM))
+
+
+inline_for_extraction noextract
+val bn_mod_exp_fw_mont_f: #t:limb_t -> k:BM.mont t -> bn_mod_exp_fw_mont_f_st t k.BM.bn.BN.len
+let bn_mod_exp_fw_mont_f #t k n mu bBits bLen b l table_len table i accM =
+  bn_mod_exp_pow2_mont_in_place k n mu l accM;
+  let bits_l = BN.bn_get_bits bLen b (bBits -! l *! i -! l) l in
+  let h0 = ST.get () in
+  SN.bn_get_bits_lemma (as_seq h0 b) (v bBits - v l * v i - v l) (v l);
+  assert (v bits_l < v table_len);
+
+  let bits_l32 = Lib.RawIntTypes.(size_from_UInt32 (u32_to_UInt32 (to_u32 bits_l))) in
+  assert (v bits_l32 == v bits_l);
+  [@inline_let] let len = k.BM.bn.BN.len in
+  Math.Lemmas.lemma_mult_le_right (v len) (v bits_l32 + 1) (v table_len);
+  let a_powbits_l = sub table (bits_l32 *! len) len in
+  k.BM.mul n mu accM a_powbits_l accM
+
+
+inline_for_extraction noextract
+let bn_mod_exp_fw_mont_rem_st (t:limb_t) (len:BN.meta_len t) =
+    n:lbignum t len
+  -> mu:limb t
+  -> bBits:size_t{0 < v bBits}
+  -> bLen:size_t{bLen == blocks bBits (size (bits t))}
+  -> b:lbignum t bLen
+  -> l:size_t{0 < v l /\ v l <= bits t}
+  -> table_len:size_t{1 < v table_len /\ v table_len * v len <= max_size_t /\ v table_len == pow2 (v l)}
+  -> table:lbignum t (table_len *! len)
+  -> accM:lbignum t len ->
+  Stack unit
+  (requires fun h ->
+    live h n /\ live h b /\ live h table /\ live h accM /\
+    disjoint accM table /\ disjoint accM b /\ disjoint accM n /\
+    disjoint accM n /\ disjoint accM b)
+  (ensures  fun h0 _ h1 -> modifies (loc accM) h0 h1 /\
+    as_seq h1 accM == S.bn_mod_exp_fw_mont_rem (as_seq h0 n) mu (v bBits) (v bLen) (as_seq h0 b)
+      (v l) (v table_len) (as_seq h0 table) (as_seq h0 accM))
+
+
+inline_for_extraction noextract
+val bn_mod_exp_fw_mont_rem: #t:limb_t -> k:BM.mont t -> bn_mod_exp_fw_mont_rem_st t k.BM.bn.BN.len
+let bn_mod_exp_fw_mont_rem #t k n mu bBits bLen b l table_len table accM =
+  let c = bBits %. l in
+  assert (v c == v bBits % v l);
+  bn_mod_exp_pow2_mont_in_place k n mu c accM;
+  let bits_c = BN.bn_get_bits bLen b 0ul c in
+  let h0 = ST.get () in
+  SN.bn_get_bits_lemma (as_seq h0 b) 0 (v c);
+  Math.Lemmas.pow2_lt_compat (v l) (v c);
+  assert (v bits_c < v table_len);
+
+  let bits_c32 = Lib.RawIntTypes.(size_from_UInt32 (u32_to_UInt32 (to_u32 bits_c))) in
+  assert (v bits_c32 == v bits_c);
+  [@inline_let] let len = k.BM.bn.BN.len in
+  Math.Lemmas.lemma_mult_le_right (v len) (v bits_c32 + 1) (v table_len);
+  let a_powbits_l = sub table (bits_c32 *! len) len in
+  k.BM.mul n mu accM a_powbits_l accM
+
+
+inline_for_extraction noextract
+let bn_mod_exp_fw_mont_loop_st (t:limb_t) (len:BN.meta_len t) =
+    n:lbignum t len
+  -> mu:limb t
+  -> bBits:size_t{0 < v bBits}
+  -> bLen:size_t{bLen == blocks bBits (size (bits t))}
+  -> b:lbignum t bLen
+  -> l:size_t{0 < v l /\ v l <= bits t /\ pow2 (v l) * v len <= max_size_t}
+  -> table_len:size_t{1 < v table_len /\ v table_len * v len <= max_size_t /\ v table_len == pow2 (v l)}
+  -> table:lbignum t (table_len *! len)
+  -> accM:lbignum t len ->
+  Stack unit
+  (requires fun h ->
+    live h n /\ live h b /\ live h accM /\ live h table /\
+    disjoint accM b /\ disjoint accM n /\ disjoint accM table /\ disjoint n table)
+  (ensures  fun h0 _ h1 -> modifies (loc accM) h0 h1 /\
+    as_seq h1 accM ==
+    Loops.repeati (v bBits / v l) (S.bn_mod_exp_fw_mont_f (as_seq h0 n) mu
+      (v bBits) (v bLen) (as_seq h0 b) (v l) (v table_len) (as_seq h0 table)) (as_seq h0 accM))
+
+
+inline_for_extraction noextract
+val bn_mod_exp_fw_mont_loop: #t:limb_t -> k:BM.mont t -> bn_mod_exp_fw_mont_loop_st t k.BM.bn.BN.len
+let bn_mod_exp_fw_mont_loop #t k n mu bBits bLen b l table_len table accM = admit();
+  [@inline_let]
+  let spec h0 = S.bn_mod_exp_fw_mont_f (as_seq h0 n) mu
+      (v bBits) (v bLen) (as_seq h0 b) (v l) (v table_len) (as_seq h0 table) in
+  let h0 = ST.get () in
+  let it = bBits /. l in
+  assert (v it == v bBits / v l);
+  Math.Lemmas.multiply_fractions (v bBits) (v l);
+
+  loop1 h0 it accM spec
+  (fun i ->
+    Loops.unfold_repeati (v it) (spec h0) (as_seq h0 accM) (v i);
+    bn_mod_exp_fw_mont_f k n mu bBits bLen b l table_len table i accM
+  )
+
+
+inline_for_extraction noextract
+let bn_mod_exp_fw_mont_aux_st (t:limb_t) (len:BN.meta_len t) =
+    n:lbignum t len
+  -> mu:limb t
+  -> aM:lbignum t len
+  -> bBits:size_t{0 < v bBits}
+  -> b:lbignum t (blocks bBits (size (bits t)))
+  -> l:size_t{0 < v l /\ v l < bits U32 /\ pow2 (v l) * v len <= max_size_t}
+  -> r2:lbignum t len
+  -> resM:lbignum t len ->
+  Stack unit
+  (requires fun h ->
+    live h n /\ live h b /\ live h aM /\ live h resM /\ live h r2 /\
+    disjoint resM aM /\ disjoint resM b /\ disjoint resM n /\
+    disjoint resM r2 /\ disjoint aM n /\
+    disjoint aM b /\ disjoint aM r2 /\ disjoint n r2)
+  (ensures  fun h0 _ h1 -> modifies (loc resM) h0 h1 /\
+    as_seq h1 resM == S.bn_mod_exp_fw_mont_ (as_seq h0 n) mu (as_seq h0 aM) (v bBits) (as_seq h0 b) (v l) (as_seq h0 r2))
+
+
+inline_for_extraction noextract
+val bn_mod_exp_fw_mont_aux: #t:limb_t -> k:BM.mont t -> bn_mod_exp_fw_mont_aux_st t k.BM.bn.BN.len
+let bn_mod_exp_fw_mont_aux #t k n mu aM bBits b l r2 accM =
+  [@inline_let] let len = k.BM.bn.BN.len in
+  let bLen = blocks bBits (size (bits t)) in
+  push_frame ();
+  let acc = create len (uint #t #SEC 0) in
+  BN.bn_from_uint len (uint #t 1) acc;
+  k.BM.to n mu r2 acc accM;
+
+  let table_len = 1ul <<. l in
+  assert (v table_len == pow2 (v l));
+  Math.Lemmas.pow2_le_compat (v l) 1;
+  assert (1 < v table_len /\ v table_len * v len <= max_size_t);
+  let table = create (table_len *! len) (uint #t #SEC 0) in
+  bn_mod_precomp_table_mont k n mu table_len aM accM table;
+
+  bn_mod_exp_fw_mont_loop #t k n mu bBits bLen b l table_len table accM;
+
+  if bBits %. l <>. 0ul then
+    bn_mod_exp_fw_mont_rem k n mu bBits bLen b l table_len table accM;
+  pop_frame()
+
+
+let bn_mod_exp_fw_precompr2 #t k n a bBits b l r2 res =
+  [@inline_let] let len = k.BM.bn.BN.len in
+  push_frame ();
+  let mu = BM.mod_inv_limb n.(0ul) in
+  let aM = create len (uint #t #SEC 0) in
+  k.BM.to n mu r2 a aM;
+
+  let resM = create len (uint #t #SEC 0) in
+  bn_mod_exp_fw_mont_aux #t k n mu aM bBits b l r2 resM;
+  k.BM.from n mu resM res;
+  pop_frame ()
+
+
+let bn_mod_exp_fw #t k bn_mod_exp_fw_precompr2 nBits n a bBits b l res =
+  [@inline_let] let len = k.BM.bn.BN.len in
+  push_frame ();
+  let r2 = create len (uint #t #SEC 0) in
+  BM.precomp nBits n r2;
+  bn_mod_exp_fw_precompr2 n a bBits b l r2 res;
+  pop_frame ()
